update

theories/Core/Contract.v
@@ -10,11 +10,6 @@ Require Import Setoid.
 Require Import Init.Tauto btauto.Btauto.
 Require Import Logic.ClassicalFacts.
 
-(** printing =~ %$=\sim$% *)
-
-(* Set Implicit Arguments. *)
-
-
 Inductive EventType : Type :=
 | Transfer : EventType
 | Notify : EventType.
@@ -23,6 +18,12 @@ Scheme Equality for EventType.
 
 Definition Trace := List.list EventType % type.
 
+Lemma plus_minus2 : forall (n0 n1 : nat), n0 + n1 = n1 + n0.
+Proof.
+induction n0;intros;simpl.
+- induction n1; [ | simpl; rewrite <- IHn1]; reflexivity. 
+- rewrite IHn0. rewrite plus_n_Sm. reflexivity. 
+Qed.
 
 Inductive Contract : Set :=
 | Success : Contract
@@ -51,31 +52,7 @@ match c with
 | c0 _;_ c1 => nu c0 && nu c1
 | c0 _+_ c1 => nu c0 || nu c1
 end.
-(*
-Definition o (c : Contract) := if nu c then Success else Failure.
-Hint Unfold o : core.
 
-Lemma o_Failure : o Failure = Failure.
-Proof. reflexivity.
-Qed.
-
-Lemma o_Success : o Success = Success.
-Proof. reflexivity.
-Qed.
-
-
-Lemma o_or : forall (c : Contract), o c = Success /\ nu c = true \/ o c = Failure /\ nu c = false.
-Proof.
-intros. unfold o. destruct (nu c) eqn:Heqn; intuition.
-Qed.
-
-Lemma o_idempotent : forall (c : Contract), o (o c) = o c.
-Proof.
-intros. destruct (o_or c). destruct H. rewrite H;auto. destruct H. now rewrite H. 
-Qed.
-
-Hint Rewrite o_Failure o_Success o_idempotent : cDB.
-*)
 
 Reserved Notation "e \ c" (at level 40, left associativity).
 Fixpoint derive (e:EventType) (c:Contract) :Contract :=
@@ -95,37 +72,8 @@ Ltac destruct_ctx :=
          | [ H: ?H0 /\ ?H1 |- _ ] => destruct H
          | [ H: exists _, _  |- _ ] => destruct H
          end.
-(*
-Ltac o_destruct :=
-  match goal with
-         | [ |- context[(o ?c)] ] => destruct (o_or c);destruct_ctx
-         | [ _ : context[ (o ?c)] |- _ ] => let H := fresh "H" in 
-                                            let H1 := fresh "H1" in 
-                                            destruct (o_or c) as [[H H1] | [H H1]];
-                                            rewrite H in*;clear H
-         end.*)
-(*
-Lemma o_derive : forall c e, e \ (o c) = Failure.
-Proof.
-intros. o_destruct. unfold o. rewrite H0. now simpl. unfold o. rewrite H0. now simpl.
-Qed.
 
-Hint Rewrite o_idempotent o_derive : cDB.*)
 Ltac autoIC := auto with cDB.
-
-
-(*Removed because it is not needed in this file*)
-(*
-Inductive Trace_Derive : Contract -> Trace -> Contract -> Prop :=
-| Trace_Derive_Nil c : Trace_Derive c [] c
-| Trace_Derive_Cons c s c' e (H: Trace_Derive (c/e) s c') : Trace_Derive c (e::s) c'. (*rule motivated by constructor being analgous to cons on lists*)
-Hint Constructors Trace_Derive : cDB.
-
-
-Lemma Trace_Derive_trans : forall s s' c0 c1 c2 , Trace_Derive c0 s c1 -> Trace_Derive c1 s' c2 -> Trace_Derive c0 (s++s') c2.
-Proof.
-intros. induction H;simpl;autoIC.
-Qed.*)
 
 
 Reserved Notation "s \\ c" (at level 42, no associativity).
@@ -136,93 +84,56 @@ match s with
 end
 where "s \\ c" := (trace_derive s c).
 
-(*
-Lemma trace_derive_spec : forall (c c' : Contract)(s : Trace), c // s = c' <-> Trace_Derive c s c'.
-Proof.
-split;intros.
-- funelim (trace_derive c s);simpl;autoIC.
-- induction H;auto. 
-Qed.
-
-Lemma trace_derive_spec2 : forall (c : Contract)(s : Trace), Trace_Derive c s (c // s).
-Proof.
-intros. remember (c//s). symmetry in Heqc0. now rewrite <- trace_derive_spec.
-Qed.*)
-
-
 Definition matchesb (c : Contract)(s : Trace) := nu (s\\c).
 
 
-Reserved Notation "s =~ re" (at level 63).
+Reserved Notation "s (:) re" (at level 63).
 
 Inductive Matches_Comp : Trace -> Contract -> Prop :=
-  | MSuccess : [] =~ Success
-  | MEvent x : [x] =~ (Event x)
+  | MSuccess : Matches_Comp [] Success
+  | MEvent x : Matches_Comp [x] (Event x)
   | MSeq s1 c1 s2 c2
-             (H1 : s1 =~ c1)
-             (H2 : s2 =~ c2)
-           : (s1 ++ s2) =~ (c1 _;_ c2)
+             (H1 : Matches_Comp s1 c1)
+             (H2 : Matches_Comp s2 c2)
+           : Matches_Comp (s1 ++ s2) (c1 _;_ c2)
   | MPlusL s1 c1 c2
-                (H1 : s1 =~ c1)
-              : s1 =~ (c1 _+_ c2)
+                (H1 : Matches_Comp s1 c1)
+              : Matches_Comp s1 (c1 _+_ c2)
   | MPlusR c1 s2 c2
-                (H2 : s2 =~ c2)
-              : s2 =~ (c1 _+_ c2)
- (* | MStar0 c 
-              : [] =~ Star c
-  | MStarSeq c s1 s2 (H1: s1 =~ c) 
-                     (H2: s2 =~ Star c) 
-              : s1 ++ s2 =~ Star c*)
-  where "s =~ c" := (Matches_Comp s c).
+                (H2 : Matches_Comp s2 c2)
+              : Matches_Comp s2 (c1 _+_ c2).
 
-(*Derive Signature for Matches_Comp.*)
+Notation "s (:) c" := (Matches_Comp s c)(at level 63).
+
 
 Hint Constructors Matches_Comp : cDB.
 
 Ltac eq_event_destruct :=
   repeat match goal with
-         | [ |- context[EventType_eq_dec ?e ?e0] ] => destruct (EventType_eq_dec e e0);try contradiction
-         | [ _ : context[EventType_eq_dec ?e ?e0]  |- _ ] => destruct (EventType_eq_dec e e0);try contradiction
+         | [ |- context[EventType_eq_dec ?e ?e0] ] 
+                => destruct (EventType_eq_dec e e0);try contradiction
+         | [ _ : context[EventType_eq_dec ?e ?e0]  |- _ ] 
+                => destruct (EventType_eq_dec e e0);try contradiction
          end.
 
-Lemma seq_Success : forall c s, s =~ Success _;_ c <-> s =~ c.
+Lemma seq_Success : forall c s, s (:) Success _;_ c <-> s (:) c.
 Proof.
 split;intros. inversion H. inversion H3. subst. now simpl.
 rewrite <- (app_nil_l s). autoIC.
 Qed. 
 
-Lemma seq_Failure : forall c s, s =~ Failure _;_ c <-> s =~ Failure.
+Lemma seq_Failure : forall c s, s (:) Failure _;_ c <-> s (:) Failure.
 Proof.
 split;intros. inversion H. inversion H3. inversion H.
 Qed.
 
 Hint Resolve seq_Success seq_Failure : cDB.
 
-(*
-Lemma o_or : forall (c0 c1 : Contract)(s : Trace), s =~ o c0 _;_ c1 -> nu c0 = true /\ s =~ c1 \/ nu c0 = false /\ s =~ Failure.
-Proof.
-intros. o_destruct. unfold o in H. destruct (nu c0). funelim (o c0).
-- rewrite <- Heqcall in H. rewrite seq_Success in H. now left.
-- rewrite <- Heqcall in H. rewrite seq_Failure in H. now right.
-Qed.*)
-
-Lemma derive_distr_plus : forall (s : Trace)(c0 c1 : Contract), s \\ (c0 _+_ c1) = s \\ c0 _+_ s \\ c1.
+Lemma derive_distr_plus : forall (s : Trace)(c0 c1 : Contract), 
+s \\ (c0 _+_ c1) = s \\ c0 _+_ s \\ c1.
 Proof.
 induction s;intros;simpl;auto.
 Qed. 
-(*
-Check existsb.
-(*Lemma nu_derive_disjuncts_seq : forall s c0 c1, nu (s \\ (c0 _;_ c1)) = existsb (fun ss => nu ((fst ss) \\ c0) && nu (snd ss) \\ c1)*)
-
-Lemma o_true : forall (c: Contract), nu c = true -> o c = Success.
-Proof.
-intros. o_destruct;auto with cDB. rewrite H in H1. discriminate. 
-Qed.
-
-Lemma o_false : forall (c: Contract), nu c = false -> o c = Failure.
-Proof.
-intros. o_destruct. rewrite H in H1. discriminate. auto. 
-Qed.*)
 
 Hint Rewrite derive_distr_plus : cDB.
 
@@ -232,21 +143,17 @@ Proof.
 intros. simpl. destruct (nu c0). simpl. auto with bool. discriminate.
 Qed.
 
-(*Not needed*)
-(*
-Lemma nu_plus : forall c0 c1, nu (c0 _+_ c1) = true <-> nu c0 = true \/ nu c1 = true.
-Proof.
-intros. simpl. now rewrite orb_true_iff.
-Qed.*)
 
-Lemma nu_Failure : forall (s : Trace)(c : Contract), nu (s \\ (Failure _;_ c)) = false.
+Lemma nu_Failure : forall (s : Trace)(c : Contract), 
+nu (s \\ (Failure _;_ c)) = false.
 Proof.
 induction s;intros. now simpl. simpl. auto.
 Qed.
 
 Hint Rewrite nu_Failure : cDB.
 
-Lemma nu_Success : forall (s : Trace)(c : Contract), nu (s \\ (Success _;_ c)) = nu (s \\ c).
+Lemma nu_Success : forall (s : Trace)(c : Contract), 
+nu (s \\ (Success _;_ c)) = nu (s \\ c).
 Proof.
 induction s;intros;simpl;auto. 
 autorewrite with cDB using simpl;auto.
@@ -261,7 +168,8 @@ induction s;intros;simpl in *. intuition. destruct (nu c0).
 rewrite derive_distr_plus. simpl. auto with bool. discriminate.
 Qed.
 
-Lemma matchesb_seq : forall (s0 s1 : Trace)(c0 c1 : Contract), nu (s0\\c0) = true -> nu (s1\\c1) = true -> nu ((s0++s1)\\(c0 _;_c1)) = true.
+Lemma matchesb_seq : forall (s0 s1 : Trace)(c0 c1 : Contract), 
+nu (s0\\c0) = true -> nu (s1\\c1) = true -> nu ((s0++s1)\\(c0 _;_c1)) = true.
 Proof.
 induction s0;intros;simpl in *.
 - rewrite nu_seq_trace_derive; auto. 
@@ -270,27 +178,28 @@ Qed.
 
 Hint Rewrite matchesb_seq : cDB.
 
-Lemma Matches_Comp_i_matchesb : forall (c : Contract)(s : Trace), s =~ c -> nu (s\\c) = true.
+Lemma Matches_Comp_i_matchesb : forall (c : Contract)(s : Trace), 
+s (:) c -> nu (s\\c) = true.
 Proof.
 intros; induction H; 
 solve [ autorewrite with cDB; simpl; auto with bool 
       | simpl;eq_event_destruct;auto ].
 Qed.
 
-Lemma Matches_Comp_nil_nu : forall (c : Contract), nu c = true -> [] =~ c.
+Lemma Matches_Comp_nil_nu : forall (c : Contract), nu c = true -> [] (:) c.
 Proof.
-intros;induction c; simpl in H ; try discriminate; autoIC. apply orb_prop in H. destruct H; autoIC.
+intros;induction c; simpl in H ; try discriminate; autoIC. 
+apply orb_prop in H. destruct H; autoIC.
 rewrite <- (app_nil_l []); autoIC.
 Qed.
 
 
-
-(*This direction with longer trace on the right because of induction step on trace*)
-Lemma Matches_Comp_derive : forall (c : Contract)(e : EventType)(s : Trace), s =~ e \ c-> (e::s) =~ c.
+Lemma Matches_Comp_derive : forall (c : Contract)(e : EventType)(s : Trace), 
+s (:) e \ c-> (e::s) (:) c.
 Proof.
 induction c;intros; simpl in*; try solve [inversion H].
 - eq_event_destruct. inversion H. subst. autoIC. inversion H.
-- inversion H; autoIC. (*apply IH directly*) 
+- inversion H; autoIC.
 - destruct (nu c1) eqn:Heqn.
   * inversion H.
     ** inversion H2. subst. rewrite app_comm_cons. auto with cDB.
@@ -300,9 +209,8 @@ induction c;intros; simpl in*; try solve [inversion H].
 Qed.
 
 
-
-
-Theorem Matches_Comp_iff_matchesb : forall (c : Contract)(s : Trace), s =~ c <-> nu (s \\ c) = true.
+Theorem Matches_Comp_iff_matchesb : forall (c : Contract)(s : Trace), 
+s (:) c <-> nu (s \\ c) = true.
 Proof.
 split;intros.
 - auto using Matches_Comp_i_matchesb.
