theories/Core/ContractEquations.v
@@ -1,7 +1,7 @@
 Require Import CSL.Core.Contract.  
 Require Import Lists.List Bool.Bool Bool.Sumbool Setoid Coq.Arith.PeanoNat.
 
-(** printing =~ %$=\sim$% *)
+(** printing (:) %$=\sim$% *)
 
 (** printing _+_ %$+$% *)
 
@@ -9,26 +9,39 @@ Import ListNotations.
 
 Set Implicit Arguments.
 
-Reserved Notation "c0 =R= c1" (at level 63).
+Reserved Notation "c0 == c1" (at level 63).
 
 Inductive c_eq : Contract -> Contract -> Prop :=
-  | c_plus_assoc c0 c1 c2 : (c0 _+_ c1) _+_ c2 =R= c0 _+_ (c1 _+_ c2)
-  | c_plus_comm c0 c1: c0 _+_ c1 =R= c1 _+_ c0
-  | c_plus_neut c: c _+_ Failure =R= c
-  | c_plus_idemp c : c _+_ c =R= c 
-  | c_seq_assoc c0 c1 c2 : (c0 _;_ c1) _;_ c2 =R= c0 _;_ (c1 _;_ c2)
-  | c_seq_neut_l c : (Success _;_ c) =R= c 
-  | c_seq_neut_r c : c _;_ Success =R= c 
-  | c_seq_failure_l c : Failure _;_ c =R= Failure    (*EXTRA AXIOM*)
-  | c_seq_failure_r c :  c _;_ Failure =R= Failure 
-  | c_distr_l c0 c1 c2 : c0 _;_ (c1 _+_ c2) =R= (c0 _;_ c1) _+_ (c0 _;_ c2)
-  | c_distr_r c0 c1 c2 : (c0 _+_ c1) _;_ c2 =R= (c0 _;_ c2) _+_ (c1 _;_ c2)
-  | c_refl c : c =R= c
-  | c_sym c0 c1 (H: c0 =R= c1) : c1 =R= c0
-  | c_trans c0 c1 c2 (H1 : c0 =R= c1) (H2 : c1 =R= c2) : c0 =R= c2
-  | c_plus_ctx c0 c0' c1 c1' (H1 : c0 =R= c0') (H2 : c1 =R= c1') : c0 _+_ c1 =R= c0' _+_ c1'
-  | c_seq_ctx c0 c0' c1 c1' (H1 : c0 =R= c0') (H2 : c1 =R= c1') : c0 _;_ c1 =R= c0' _;_ c1'
-  where "c1 =R= c2" := (c_eq c1 c2).
+  | c_plus_assoc c0 c1 c2 : 
+        (c0 _+_ c1) _+_ c2 == c0 _+_ (c1 _+_ c2)
+  | c_plus_comm c0 c1: 
+        c0 _+_ c1 == c1 _+_ c0
+  | c_plus_neut c: c _+_ Failure == c
+  | c_plus_idemp c : c _+_ c == c 
+  | c_seq_assoc c0 c1 c2 : 
+        (c0 _;_ c1) _;_ c2 == c0 _;_ (c1 _;_ c2)
+  | c_seq_neut_l c : 
+        (Success _;_ c) == c 
+  | c_seq_neut_r c : 
+        c _;_ Success == c 
+  | c_seq_failure_l c : 
+       Failure _;_ c == Failure 
+  | c_seq_failure_r c :  
+       c _;_ Failure == Failure 
+  | c_distr_l c0 c1 c2 : 
+      c0 _;_ (c1 _+_ c2) == (c0 _;_ c1) _+_ (c0 _;_ c2)
+  | c_distr_r c0 c1 c2 : 
+     (c0 _+_ c1) _;_ c2 == (c0 _;_ c2) _+_ (c1 _;_ c2)
+  | c_refl c : c == c
+  | c_sym c0 c1 (H: c0 == c1) : c1 == c0
+  | c_trans c0 c1 c2 (H1 : c0 == c1) (H2 : c1 == c2) : c0 == c2
+  | c_plus_ctx c0 c0' c1 c1' (H1 : c0 == c0') 
+                             (H2 : c1 == c1') : 
+                             c0 _+_ c1 == c0' _+_ c1'
+  | c_seq_ctx c0 c0' c1 c1' (H1 : c0 == c0') 
+                            (H2 : c1 == c1') : 
+                             c0 _;_ c1 == c0' _;_ c1'
+  where "c1 == c2" := (c_eq c1 c2).
 
 Hint Constructors c_eq : eqDB.
 
@@ -53,20 +66,22 @@ Qed.
 
 Ltac c_inversion :=
   (repeat match goal with
-         | [ H: _ =~ Failure |- _ ] => inversion H
-         | [ H: ?s =~ _ _+_ _ |- _ ] => inversion H; clear H
-         | [ H: ?s =~ _ _;_ _ |- _ ] => inversion H; clear H
-         | [ H: [?x] =~ Event _ |- _ ] => fail
-         | [ H: ?s =~ Event _ |- _ ] => inversion H; subst
-         | [ H: [] =~ Success |- _ ] => fail
-         | [ H: _ =~ Success |- _ ] => inversion H; clear H
+         | [ H: _ (:) Failure |- _ ] => inversion H
+         | [ H: ?s (:) _ _+_ _ |- _ ] => inversion H; clear H
+         | [ H: ?s (:) _ _;_ _ |- _ ] => inversion H; clear H
+         | [ H: [?x] (:) Event _ |- _ ] => fail
+         | [ H: ?s (:) Event _ |- _ ] => inversion H; subst
+         | [ H: [] (:) Success |- _ ] => fail
+         | [ H: _ (:) Success |- _ ] => inversion H; clear H
          end);auto with cDB.
 
 
-
-Lemma c_eq_soundness : forall (c0 c1 : Contract), c0 =R= c1 -> (forall s : Trace, s =~ c0 <-> s =~ c1).
+Print incl.
+Lemma c_eq_soundness : forall (c0 c1 : Contract), 
+c0 == c1 -> (forall s : Trace, s (:) c0 <-> s (:) c1).
 Proof.
-intros c0 c1 H. induction H ;intros; try solve [split;intros;c_inversion].
+intros c0 c1 H. induction H ;intros; 
+try solve [split;intros;c_inversion].
   * split;intros;c_inversion; [ rewrite <- app_assoc | rewrite app_assoc ]; auto with cDB.
   * rewrite <- (app_nil_l s). split;intros;c_inversion.
   * rewrite <- (app_nil_r s) at 1. split;intros;c_inversion. subst.
@@ -84,22 +99,22 @@ intros c0 c1 H. induction H ;intros; try solve [split;intros;c_inversion].
                                 | rewrite IHc_eq2];auto.
 Qed.
 
-Lemma Matches_plus_comm : forall c0 c1 s, s =~ c0 _+_ c1 <-> s =~ c1 _+_ c0.
+Lemma Matches_plus_comm : forall c0 c1 s, s (:) c0 _+_ c1 <-> s (:) c1 _+_ c0.
 Proof. auto using c_eq_soundness  with eqDB. Qed.
 
-Lemma Matches_plus_neut_l : forall c s, s =~ Failure _+_ c <-> s =~ c.
+Lemma Matches_plus_neut_l : forall c s, s (:) Failure _+_ c <-> s (:) c.
 Proof. intros. rewrite Matches_plus_comm. auto using c_eq_soundness  with eqDB. Qed.
 
-Lemma Matches_plus_neut_r : forall c s, s =~ c _+_ Failure <-> s =~ c.
+Lemma Matches_plus_neut_r : forall c s, s (:) c _+_ Failure <-> s (:) c.
 Proof. auto using c_eq_soundness  with eqDB. Qed.
 
-Lemma Matches_seq_neut_l : forall c s, s =~ (Success _;_ c) <-> s =~ c.
+Lemma Matches_seq_neut_l : forall c s, s (:) (Success _;_ c) <-> s (:) c.
 Proof. auto using c_eq_soundness  with eqDB. Qed.
 
-Lemma Matches_seq_neut_r : forall c s, s =~ c _;_ Success <-> s =~ c.
+Lemma Matches_seq_neut_r : forall c s, s (:) c _;_ Success <-> s (:) c.
 Proof. auto using c_eq_soundness  with eqDB. Qed.
 
-Lemma Matches_seq_assoc : forall c0 c1 c2 s, s =~ (c0 _;_ c1) _;_ c2  <-> s =~ c0 _;_ (c1 _;_ c2).
+Lemma Matches_seq_assoc : forall c0 c1 c2 s, s (:) (c0 _;_ c1) _;_ c2  <-> s (:) c0 _;_ (c1 _;_ c2).
 Proof. auto using c_eq_soundness  with eqDB. Qed.
 
 Hint Rewrite Matches_plus_neut_l 
@@ -107,7 +122,7 @@ Hint Rewrite Matches_plus_neut_l
              Matches_seq_neut_l
              Matches_seq_neut_r : eqDB.
 
-Lemma c_plus_neut_l : forall c, Failure _+_ c =R= c.
+Lemma c_plus_neut_l : forall c, Failure _+_ c == c.
 Proof. intros. rewrite c_plus_comm. auto with eqDB.
 Qed.
 
@@ -133,13 +148,13 @@ match c with
 end.
 
 
-Lemma Matches_member : forall (s : Trace)(c : Contract), s =~ c -> In s (L c). 
+Lemma Matches_member : forall (s : Trace)(c : Contract), s (:) c -> In s (L c). 
 Proof.
 intros. induction H ; simpl ; try solve [auto using in_or_app || auto using in_or_app ].
 rewrite in_map_iff. exists (s1,s2). rewrite in_prod_iff. split;auto.
 Qed.
 
-Lemma member_Matches : forall (c : Contract)(s : Trace), In s (L c) -> s =~ c. 
+Lemma member_Matches : forall (c : Contract)(s : Trace), In s (L c) -> s (:) c. 
 Proof.
 induction c;intros;simpl in*; try solve [ destruct H;try contradiction; subst; constructor].
 - apply in_app_or in H. destruct H; auto with cDB.
@@ -148,19 +163,19 @@ induction c;intros;simpl in*; try solve [ destruct H;try contradiction; subst; c
   subst. auto with cDB.
 Qed.
 
-Theorem Matches_iff_member : forall s c, s =~ c <-> In s (L c).
+Theorem Matches_iff_member : forall s c, s (:) c <-> In s (L c).
 Proof.
 split; auto using Matches_member,member_Matches.
 Qed.
 
-Lemma Matches_incl : forall (c0 c1 : Contract), (forall (s : Trace), s =~ c0 -> s =~ c1) -> 
+Lemma Matches_incl : forall (c0 c1 : Contract), (forall (s : Trace), s (:) c0 -> s (:) c1) -> 
 incl (L c0) (L c1).
 Proof.
 intros. unfold incl. intros. rewrite <- Matches_iff_member in *. auto.
 Qed.
 
-Lemma comp_equiv_destruct : forall (c0 c1: Contract),(forall s : Trace, s =~ c0 <-> s =~ c1) <->
-(forall s : Trace, s =~ c0 -> s =~ c1) /\ (forall s : Trace, s =~ c1 -> s =~ c0).
+Lemma comp_equiv_destruct : forall (c0 c1: Contract),(forall s : Trace, s (:) c0 <-> s (:) c1) <->
+(forall s : Trace, s (:) c0 -> s (:) c1) /\ (forall s : Trace, s (:) c1 -> s (:) c0).
 Proof.
  split ; intros.
 - split;intros; specialize H with s; destruct H; auto.
@@ -168,7 +183,7 @@ Proof.
 Qed.
 
 
-Theorem Matches_eq_i_incl_and : forall (c0 c1 : Contract), (forall (s : Trace), s =~ c0 <-> s =~ c1) -> 
+Theorem Matches_eq_i_incl_and : forall (c0 c1 : Contract), (forall (s : Trace), s (:) c0 <-> s (:) c1) -> 
 incl (L c0) (L c1) /\ incl (L c1) (L c0) .
 Proof.
 intros. apply comp_equiv_destruct in H. destruct H. split; auto using Matches_incl. 
@@ -183,15 +198,15 @@ end.
 
 (*Maybe not needed*)
 Lemma Σ_app : forall (l1 l2 : list Contract), 
-Σ (l1 ++ l2) =R= (Σ l1) _+_ (Σ l2).
+Σ (l1 ++ l2) == (Σ l1) _+_ (Σ l2).
 Proof.
 induction l1;intros;simpl;auto_rwd_eqDB.
 rewrite IHl1. now rewrite c_plus_assoc.
 Qed.
 
 (*Not used in this file, maybe used in decision procedure*)
-Lemma in_Σ : forall (l : list Contract)(s : Trace), s =~ Σ l <-> 
-(exists c, In c l /\ s =~ c).
+Lemma in_Σ : forall (l : list Contract)(s : Trace), s (:) Σ l <-> 
+(exists c, In c l /\ s (:) c).
 Proof. 
 induction l;intros;simpl.
 - split;intros. c_inversion. destruct_ctx. contradiction.
@@ -201,7 +216,7 @@ induction l;intros;simpl.
   apply MPlusR. rewrite IHl. exists x. split;auto.
 Qed.
 
-Lemma in_Σ_idemp : forall l c, In c l -> c _+_ Σ l =R= Σ l.
+Lemma in_Σ_idemp : forall l c, In c l -> c _+_ Σ l == Σ l.
 Proof.
 induction l;intros;simpl; auto_rwd_eqDB.
 simpl in H;contradiction.
@@ -210,21 +225,21 @@ auto_rwd_eqDB. rewrite (c_plus_comm c). rewrite c_plus_assoc.
 apply c_plus_ctx;auto_rwd_eqDB.
 Qed. 
 
-Lemma incl_Σ_idemp : forall (l1 l2 : list Contract), incl l1 l2 -> Σ l2 =R= Σ (l1++l2).
+Lemma incl_Σ_idemp : forall (l1 l2 : list Contract), incl l1 l2 -> Σ l2 == Σ (l1++l2).
 Proof. 
 induction l1;intros;simpl;auto_rwd_eqDB.
 apply incl_cons_inv in H as [H0 H1].
 rewrite <- IHl1;auto. now rewrite in_Σ_idemp;auto.
 Qed.
 
-Lemma Σ_app_comm : forall (l1 l2 : list Contract), Σ (l1++l2) =R= Σ (l2++l1).
+Lemma Σ_app_comm : forall (l1 l2 : list Contract), Σ (l1++l2) == Σ (l2++l1).
 Proof.
 induction l1;intros;simpl. now rewrite app_nil_r.
 repeat rewrite Σ_app. rewrite <- c_plus_assoc.
 rewrite c_plus_comm. apply c_plus_ctx;auto_rwd_eqDB.
 Qed.
 
-Lemma incl_Σ_c_eq : forall (l1 l2 : list Contract), incl l1 l2 -> incl l2 l1-> Σ l1 =R= Σ l2.
+Lemma incl_Σ_c_eq : forall (l1 l2 : list Contract), incl l1 l2 -> incl l2 l1-> Σ l1 == Σ l2.
 Proof.
 intros. rewrite (incl_Σ_idemp H). 
 rewrite (incl_Σ_idemp H0). apply Σ_app_comm.
@@ -237,7 +252,7 @@ match s with
 | e::s' => (Event e) _;_ (Π s')
 end.
 
-Lemma Π_app : forall (l1 l2 : Trace), Π l1 _;_ Π l2 =R= Π (l1++l2).
+Lemma Π_app : forall (l1 l2 : Trace), Π l1 _;_ Π l2 == Π (l1++l2).
 Proof.
 induction l1;intros;simpl; auto_rwd_eqDB.
 rewrite <- IHl1. auto_rwd_eqDB.
@@ -248,7 +263,7 @@ Definition Π (l : list Trace) := Σ (map Π l).
 Hint Unfold Π : eqDB.*)
 
 
-Lemma Π_distr_aux : forall (ss : list Trace) (s : Trace), Π s _;_ (Σ (map Π ss)) =R=
+Lemma Π_distr_aux : forall (ss : list Trace) (s : Trace), Π s _;_ (Σ (map Π ss)) ==
  Σ (map (fun x => Π (fst x ++ snd x)) (map (fun y : list EventType => (s, y)) ss)).
 Proof.
 induction ss;intros;simpl;auto_rwd_eqDB.
@@ -256,7 +271,7 @@ apply c_plus_ctx;auto using Π_app.
 Qed.
 
 
-Lemma Π_distr : forall l0 l1,  Σ (map Π l0) _;_ Σ (map Π l1) =R=
+Lemma Π_distr : forall l0 l1,  Σ (map Π l0) _;_ Σ (map Π l1) ==
  Σ (map (fun x => Π (fst x ++ snd x)) (list_prod l0 l1)).
 Proof.
 induction l0;intros;simpl. auto_rwd_eqDB.
@@ -267,7 +282,7 @@ Qed.
 
 
 
-Theorem Π_L_ceq : forall (c : Contract), Σ (map Π (L c)) =R= c.
+Theorem Π_L_ceq : forall (c : Contract), Σ (map Π (L c)) == c.
 Proof.
 induction c; simpl; try solve [auto_rwd_eqDB].
 - rewrite map_app. rewrite Σ_app.
@@ -279,7 +294,7 @@ Qed.
 
 
 
-Lemma c_eq_completeness : forall (c0 c1 : Contract), (forall s : Trace, s =~ c0 <-> s =~ c1) -> c0 =R= c1.
+Lemma c_eq_completeness : forall (c0 c1 : Contract), (forall s : Trace, s (:) c0 <-> s (:) c1) -> c0 == c1.
 Proof.
 intros. rewrite <- Π_L_ceq. rewrite <- (Π_L_ceq c1). 
 apply Matches_eq_i_incl_and in H.
@@ -288,7 +303,7 @@ Qed.
 
 
 
-Theorem Matches_iff_c_eq : forall c0 c1, (forall s, s =~ c0 <-> s =~ c1) <-> c0 =R= c1.
+Theorem Matches_iff_c_eq : forall c0 c1, (forall s, s (:) c0 <-> s (:) c1) <-> c0 == c1.
 Proof.
 split; auto using c_eq_completeness, c_eq_soundness.
 Qed.
